Prove CLAM/goal41

benchmarks/CLAM/goal41.v
@@ -1,28 +1,42 @@
-Require Import Nat Arith.
+Require Import Nat Arith Bool.
 
-Inductive Nat : Type := succ : Nat -> Nat |  zero : Nat.
+Inductive Nat : Type := zero : Nat | succ : Nat -> Nat.
 
-Inductive Lst : Type := cons : Nat -> Lst -> Lst |  nil : Lst.
+Scheme Equality for Nat.
+
+Inductive Lst : Type := nil : Lst | cons : Nat -> Lst -> Lst.
 
 Inductive Tree : Type := node : Nat -> Tree -> Tree -> Tree |  leaf : Tree.
 
 Inductive Pair : Type := mkpair : Nat -> Nat -> Pair
 with ZLst : Type := zcons : Pair -> ZLst -> ZLst |  znil : ZLst.
 
-Fixpoint lst_mem (lst_mem_arg0 : Nat) (lst_mem_arg1 : Lst) : bool
+Fixpoint append (append_arg0 : Lst) (append_arg1 : Lst) : Lst
+           := match append_arg0, append_arg1 with
+              | nil, x => x
+              | cons x y, z => cons x (append y z)
+              end.
+
+Fixpoint mem (mem_arg0 : Nat) (mem_arg1 : Lst) : bool
+:= match mem_arg0, mem_arg1 with
+    | x, nil => false
+    | x, cons y z => orb (Nat_beq x y) (mem x z)
+    end.
+
+Definition lst_mem (lst_mem_arg0 : Nat) (lst_mem_arg1 : Lst) : bool
            := match lst_mem_arg0, lst_mem_arg1 with
               | n, x => mem n x
               end.
 
-Fixpoint lst_subset (lst_subset_arg0 : Lst) (lst_subset_arg1 : Lst) : bool
+Fixpoint lst_subset (lst_subset_arg0 : Lst) (lst_subset_arg1 : Lst) : Prop
            := match lst_subset_arg0, lst_subset_arg1 with
-              | nil, x => true
-              | cons n x, y => andb (lst_subset x y) (lst_mem n y)
+              | nil, x => True
+              | cons n x, y => and (lst_subset x y) (lst_mem n y = true)
               end.
 
-Fixpoint lst_eq (lst_eq_arg0 : Lst) (lst_eq_arg1 : Lst) : bool
+Definition lst_eq (lst_eq_arg0 : Lst) (lst_eq_arg1 : Lst) : Prop
            := match lst_eq_arg0, lst_eq_arg1 with
-              | x, y => andb (lst_subset x y) (lst_subset y x)
+              | x, y => and (lst_subset x y) (lst_subset y x)
               end.
 
 Fixpoint lst_intersection (lst_intersection_arg0 : Lst) (lst_intersection_arg1 : Lst) : Lst
@@ -31,7 +45,48 @@ Fixpoint lst_intersection (lst_intersection_arg0 : Lst) (lst_intersection_arg1 :
               | cons n x, y => if lst_mem n y then cons n (lst_intersection x y) else lst_intersection x y
               end.
 
-Theorem theorem0 : forall (x : Lst) (y : Lst), eq (lst_subset x y) true -> eq (lst_eq (lst_intersection x y) x) true.
+Lemma Nat_beq_refl : forall (n : Nat), Nat_beq n n = true.
 Proof.
-Admitted.
+  intros.
+  induction n.
+  - reflexivity.
+  - assumption.
+Qed.
 
+Lemma append_single : forall (x : Lst) (n : Nat), cons n x = append (cons n nil) x.
+Proof.
+  reflexivity.
+Qed.
+
+Lemma mem_append : forall (n : Nat) (x y : Lst), lst_mem n x = true -> lst_mem n (append y x) = true.
+Proof.
+  intros.
+  induction y.
+  - simpl. assumption.
+  - simpl. rewrite IHy. apply orb_true_r.
+Qed.
+
+Lemma subset_append_general : forall (x y z : Lst), lst_subset x y -> lst_subset x (append z y).
+Proof.
+  intros.
+  induction x.
+  - reflexivity.
+  - simpl. simpl in H. destruct H. apply IHx in H. split.
+    + assumption.
+    + rewrite mem_append. split.
+      * assumption.
+Qed.
+
+Theorem theorem0 : forall (x : Lst) (y : Lst), lst_subset x y -> lst_eq (lst_intersection x y) x.
+Proof.
+  intros.
+  induction x.
+  - simpl. unfold lst_eq. tauto.
+  - simpl. simpl in H. destruct H. rewrite H0. apply IHx in H. unfold lst_eq in H. destruct H. unfold lst_eq. split.
+    + simpl. split.
+      * rewrite append_single. apply subset_append_general. assumption.
+      * rewrite Nat_beq_refl. reflexivity.
+    + simpl. split.
+      * rewrite append_single. apply subset_append_general. assumption.
+      * rewrite Nat_beq_refl. reflexivity.
+Qed.
